Implement mlswg/mls-protocol#587 + mlswg/mls-protocol#603 (redundant nodes)

fstar/MLS.NetworkBinder.fst
@@ -163,33 +163,53 @@ let update_path_node_to_treekem #bytes #cb group_context dir update_path_node =
     })
   )
 
+// I could use TreeKEM.tree_resolution t = [], but then I get weird errors when loading TreeSyncTreeKEMBinder...
+val tree_resolution_empty: #bytes:Type0 -> {|crypto_bytes bytes|} -> #l:nat -> #n:tree_size l -> TK.treekem bytes l n -> bool
+let rec tree_resolution_empty #bytes #cb #l #n t =
+  match t with
+  | TLeaf None -> true
+  | TLeaf (Some _) -> false
+  | TSkip _ t' -> tree_resolution_empty t'
+  | TNode None left right ->
+    tree_resolution_empty left && tree_resolution_empty right
+  | TNode (Some _) _ _ -> false
+
 #push-options "--z3rlimit 30"
-val update_path_to_treekem: #bytes:Type0 -> {|crypto_bytes bytes|} -> l:nat -> n:tree_size l -> i:leaf_index n -> bytes -> update_path:update_path_nt bytes -> result (TK.pathkem bytes l n i)
-let rec update_path_to_treekem #bytes #cb l n i group_context update_path =
-  if l = 0 then (
+val update_path_to_treekem: #bytes:Type0 -> {|crypto_bytes bytes|} -> #l:nat -> #n:tree_size l -> i:leaf_index n -> TK.treekem bytes l n -> bytes -> update_path:update_path_nt bytes -> result (TK.pathkem bytes l n i)
+let rec update_path_to_treekem #bytes #cb #l #n i t group_context update_path =
+  match t with
+  | TLeaf _ -> (
     if not (Seq.length update_path.nodes = 0) then
       internal_failure "update_path_to_treekem: update_path.nodes is too long"
     else (
       leaf_package <-- leaf_node_to_treekem update_path.leaf_node;
       return (PLeaf leaf_package)
     )
-  ) else if (n <= pow2 (l-1)) then (
-    path_next <-- update_path_to_treekem (l-1) n i group_context update_path;
+  )
+  | TSkip _ t' -> (
+    path_next <-- update_path_to_treekem i t' group_context update_path;
     return (PSkip _ path_next)
-  ) else (
+  )
+  | TNode _ left right -> (
     if not (Seq.length update_path.nodes > 0) then
       internal_failure "update_path_to_treekem: update_path.nodes is too short"
     else (
-      let update_path_length = (Seq.length update_path.nodes) in
-      let head_update_path_nodes = Seq.index update_path.nodes (update_path_length-1) in
-      let tail_update_path_nodes = Seq.slice update_path.nodes 0 (update_path_length-1) in
-      //TODO this is an easy lemma
-      assume (bytes_length ps_update_path_node_nt (Seq.seq_to_list tail_update_path_nodes) <= bytes_length ps_update_path_node_nt (Seq.seq_to_list update_path.nodes));
-      let next_update_path = { update_path with nodes = tail_update_path_nodes } in
       let (|dir, next_i|) = child_index l i in
-      path_next <-- update_path_to_treekem (l-1) (if dir = Left then pow2 (l-1) else n - (pow2 (l-1))) next_i group_context next_update_path;
-      path_data <-- update_path_node_to_treekem group_context dir head_update_path_nodes;
-      return (PNode path_data path_next)
+      let (child, sibling) = order_subtrees dir (left, right) in
+      if tree_resolution_empty sibling then (
+        path_next <-- update_path_to_treekem next_i child group_context update_path;
+        return (PNode None path_next)
+      ) else (
+        let update_path_length = (Seq.length update_path.nodes) in
+        let head_update_path_nodes = Seq.index update_path.nodes (update_path_length-1) in
+        let tail_update_path_nodes = Seq.slice update_path.nodes 0 (update_path_length-1) in
+        //TODO this is an easy lemma
+        assume (bytes_length ps_update_path_node_nt (Seq.seq_to_list tail_update_path_nodes) <= bytes_length ps_update_path_node_nt (Seq.seq_to_list update_path.nodes));
+        let next_update_path = { update_path with nodes = tail_update_path_nodes } in
+        path_next <-- update_path_to_treekem next_i child group_context next_update_path;
+        path_data <-- update_path_node_to_treekem group_context dir head_update_path_nodes;
+        return (PNode (Some path_data) path_next)
+      )
     )
   )
 #pop-options
